Started work on making exhLang have a value relation
The correctness proof into exhLang needs to use a value relation,
instead of a function on values. With a function, the proof can only
talk about the compilers current type to constructor mapping, which
makes it very hard to use the theorem to reason about the compiler for
building a REPL because the constructor mapping will be updated, and you
still need to know about the old values.

To fix the problem, values will be related if there is a submap of the
constructor mapping under which the translation from decLang to exhLang
gives the right answer. This builds the right weakening property into
the value relation, and is how things were handled in modLang and
conLang.

compiler/proofs/exhLangProofScript.sml
@@ -13,25 +13,69 @@ open compilerTerminationTheory;
 
 val _ = new_theory "exhLangProof";
 
-val v_to_exh_def = tDefine "v_to_exh" `
-(v_to_exh exh (Litv_i2 l) =
-  Litv_exh l) ∧
-(v_to_exh exh (Conv_i2 t vs) =
-  Conv_exh (FST t) (vs_to_exh exh vs)) ∧
-(v_to_exh exh (Closure_i2 env x e) =
-  Closure_exh (env_to_exh exh env) x (exp_to_exh exh e)) ∧
-(v_to_exh exh (Recclosure_i2 env funs x) =
-  Recclosure_exh (env_to_exh exh env) (funs_to_exh exh funs) x) ∧
-(v_to_exh exh (Loc_i2 l) =
-  Loc_exh l) ∧
-(vs_to_exh exh [] = []) ∧
-(vs_to_exh exh (v::vs) = v_to_exh exh v :: vs_to_exh exh vs) ∧
-(env_to_exh exh [] = []) ∧
-(env_to_exh exh ((x,v)::env) = (x,v_to_exh exh v) :: env_to_exh exh env)`
-(WF_REL_TAC`inv_image $< (\x. case x of
-  | INL (_,v) => v_i2_size v
-  | INR (INL (_,vs)) => v_i23_size vs
-  | INR (INR (_,env)) => v_i21_size env)`)
+val (v_to_exh_rules, v_to_exh_ind, v_to_exh_cases) = Hol_reln `
+(!exh l.
+  v_to_exh exh (Litv_i2 l) (Litv_exh l)) ∧
+(!exh t vs vs'.
+  vs_to_exh exh vs vs'
+  ⇒
+  v_to_exh exh (Conv_i2 t vs) (Conv_exh (FST t) vs')) ∧
+(!exh env x e env' exh'.
+  exh' SUBMAP exh ∧
+  env_to_exh exh' env env'
+  ⇒
+  v_to_exh exh (Closure_i2 env x e) (Closure_exh env' x (exp_to_exh exh' e))) ∧
+(!exh env x funs exh'.
+  exh' SUBMAP exh ∧
+  env_to_exh exh' env env'
+  ⇒
+  v_to_exh exh (Recclosure_i2 env funs x) (Recclosure_exh env' (funs_to_exh exh' funs) x)) ∧
+(!exh l.
+  v_to_exh exh (Loc_i2 l) (Loc_exh l)) ∧
+(!exh.
+  vs_to_exh exh [] []) ∧
+(!exh v v' vs vs'.
+  v_to_exh exh v v' ∧
+  vs_to_exh exh vs vs'
+  ⇒
+  vs_to_exh exh (v::vs) (v'::vs')) ∧
+(!exh.
+  env_to_exh exh [] []) ∧
+(!exh x v v' env env'.
+  v_to_exh exh v v' ∧
+  env_to_exh exh env env'
+  ⇒
+  env_to_exh exh ((x,v)::env) ((x,v')::env'))`;
+
+val v_to_exh_eqn = Q.prove (
+`(!exh l v.
+  v_to_exh exh (Litv_i2 l) v ⇔
+   v = Litv_exh l) ∧
+ (!exh t vs v.
+  v_to_exh exh (Conv_i2 t vs) v ⇔
+   ?vs'.
+    vs_to_exh exh vs vs' ∧
+    v = Conv_exh (FST t) vs') ∧
+ (!exh l.
+  v_to_exh exh (Loc_i2 l) v ⇔
+   v = Loc_exh l) ∧
+ (!exh vs. vs_to_exh exh [] vs ⇔ vs = []) ∧
+ (!exh v vs vs'. 
+  vs_to_exh exh (v::vs) vs' ⇔ 
+  ?v' vs''. 
+    vs' = v'::vs'' ∧
+    v_to_exh exh v v' ∧
+    vs_to_exh exh vs vs'') ∧
+ (!exh env. env_to_exh exh [] env ⇔ env = []) ∧
+ (!exh x v env env'.
+  env_to_exh exh ((x,v)::env) env' ⇔ 
+  ?v' env''.
+    env' = (x,v') :: env'' ∧
+    v_to_exh exh v v' ∧
+    env_to_exh exh env env'')`,
+ rw [] >>
+ rw [Once v_to_exh_cases] >>
+ metis_tac []);
 
 val store_to_exh_def = Define `
 store_to_exh exh (s,genv) =
@@ -129,9 +173,9 @@ val exh_to_exists_match = Q.prove (
      Cases_on`z`>>simp[pmatch_i2_def] >> rw[] >>
      metis_tac[pmatch_list_i2_all_vars_not_No_match]))
 
-val vs_to_exh_MAP = prove(
-  ``∀vs exh. vs_to_exh exh vs = MAP (v_to_exh exh) vs``,
-  Induct >> simp[v_to_exh_def])
+val vs_to_exh_LIST_REL = prove(
+  ``∀vs vs' exh. vs_to_exh exh vs vs' = LIST_REL (v_to_exh exh) vs vs'``,
+  Induct >> simp[v_to_exh_eqn])
 
 val funs_to_exh_MAP = prove(
   ``funs_to_exh exh ls = MAP (λ(x,y,z). (x,y,exp_to_exh exh z)) ls``,
@@ -166,32 +210,52 @@ val build_rec_env_exh_MAP = prove(
   Induct >> rw[libTheory.bind_def] >>
   PairCases_on`h` >> rw[])
 
-val env_to_exh_MAP = prove(
-  ``env_to_exh exh env = MAP (λ(x,y). (x, v_to_exh exh y)) env``,
-  Induct_on`env`>>simp[v_to_exh_def]>>Cases>>simp[v_to_exh_def])
+val env_to_exh_LIST_REL = Q.prove(
+  `!exh env env'. env_to_exh exh env env' = LIST_REL (λ(x,y) (x',y'). x = x' ∧ v_to_exh exh y y') env env'`,
+  Induct_on`env`>>simp[v_to_exh_eqn]>>Cases>>simp[v_to_exh_eqn] >>
+  rw [EXISTS_PROD]);
 
+  (*
 val env_to_exh_build_rec_env_i2 = prove(
   ``∀l1 l2 l3 exh.
     env_to_exh exh (build_rec_env_i2 l1 l2 l3) =
     build_rec_env_exh (funs_to_exh exh l1) (env_to_exh exh l2) (env_to_exh exh l3)``,
   simp[build_rec_env_i2_MAP,build_rec_env_exh_MAP,env_to_exh_MAP,funs_to_exh_MAP
-      ,MAP_MAP_o,combinTheory.o_DEF,UNCURRY,v_to_exh_def])
+      ,MAP_MAP_o,combinTheory.o_DEF,UNCURRY,v_to_exh_eqn])
+      *)
 
-val _ = augment_srw_ss[rewrites[vs_to_exh_MAP,find_recfun_funs_to_exh,env_to_exh_build_rec_env_i2]]
+val _ = augment_srw_ss[rewrites[vs_to_exh_LIST_REL,find_recfun_funs_to_exh(*,env_to_exh_build_rec_env_i2*)]]
 
-val do_eq_exh_correct = prove(
-  ``(∀v1 v2 exh.
-      do_eq_i2 v1 v2 ≠ Eq_type_error ⇒
-      do_eq_exh (v_to_exh exh v1) (v_to_exh exh v2) =
-                 do_eq_i2 v1 v2) ∧
-    (∀vs1 vs2 exh.
-      do_eq_list_i2 vs1 vs2 ≠ Eq_type_error ⇒
-      do_eq_list_exh (vs_to_exh exh vs1) (vs_to_exh exh vs2) =
-                   do_eq_list_i2 vs1 vs2)``,
-  ho_match_mp_tac do_eq_i2_ind >>
-  reverse(rw[do_eq_i2_def,do_eq_exh_def,v_to_exh_def]) >>
-  rw[] >> fs[] >> every_case_tac >> fs[] )
+val do_eq_exh_correct = Q.prove (
+`(!v1 v2 tagenv r v1_exh v2_exh exh.
+  do_eq_i2 v1 v2 = r ∧
+  v_to_exh exh v1 v1_exh ∧
+  v_to_exh exh v2 v2_exh
+  ⇒
+  do_eq_exh v1_exh v2_exh = r) ∧
+ (!vs1 vs2 tagenv r vs1_exh vs2_exh exh.
+  do_eq_list_i2 vs1 vs2 = r ∧
+  vs_to_exh exh vs1 vs1_exh ∧
+  vs_to_exh exh vs2 vs2_exh
+  ⇒
+  do_eq_list_exh vs1_exh vs2_exh = r)`,
+ ho_match_mp_tac do_eq_i2_ind >>
+ reverse(rw[do_eq_exh_def,do_eq_i2_def,v_to_exh_eqn]) >>
+ rw[v_to_exh_eqn, do_eq_exh_def] >> 
+ fs[do_eq_exh_def]
+ >- (every_case_tac >>
+     rw [] >>
+     fs [] >>
+     metis_tac [eq_result_distinct, eq_result_11]) >>
+ fs [Once v_to_exh_cases] >>
+ rw [do_eq_exh_def] >>
+ fs [] >>
+ metis_tac [LIST_REL_LENGTH]);
+ 
+  (*
 val _ = augment_srw_ss[rewrites[do_eq_exh_correct]]
+*)
+
 
 val evaluate_exh_lit = prove(
   ``evaluate_exh ck env csg (Lit_exh l) res ⇔ (res = (csg,Rval (Litv_exh l)))``,
@@ -201,24 +265,74 @@ val if_cons = prove(
   ``(if b then a::c1 else a::c2) = a::(if b then c1 else c2)``,
   rw[])
 
-val pmatch_exh_correct = prove(
-  ``(∀exh s p v env.
-      pmatch_i2 exh s p v env ≠ Match_type_error ⇒
-      pmatch_exh (MAP (v_to_exh exh) s) (pat_to_exh p) (v_to_exh exh v) (env_to_exh exh env) =
-      case pmatch_i2 exh s p v env of
-      | Match env' => Match (env_to_exh exh env')
-      | No_match => No_match) ∧
-    (∀exh s p v env.
-      pmatch_list_i2 exh s p v env ≠ Match_type_error ⇒
-      pmatch_list_exh (MAP (v_to_exh exh) s) (MAP pat_to_exh p) (vs_to_exh exh v) (env_to_exh exh env) =
-      case pmatch_list_i2 exh s p v env of
-      | Match env' => Match (env_to_exh exh env')
-      | No_match => No_match)``,
-  ho_match_mp_tac pmatch_i2_ind >>
-  simp[pmatch_i2_def,v_to_exh_def,pat_to_exh_def,pmatch_exh_def] >>
-  rw[bind_def,v_to_exh_def] >>
-  every_case_tac >> fs[ETA_AX] >>
-  fs[store_lookup_def,EL_MAP] >> rw[])
+val match_result_to_exh_def = Define
+`(match_result_to_exh exh (Match env) (Match env_exh) ⇔
+   env_to_exh exh env env_exh) ∧
+ (match_result_to_exh exh No_match No_match = T) ∧
+ (match_result_to_exh exh Match_type_error Match_type_error = T) ∧
+ (match_result_to_exh exh _ _ = F)`;
+
+val match_result_error = Q.prove (
+`(!exh r. match_result_to_exh exh r Match_type_error ⇔ r = Match_type_error) ∧
+ (!exh r. match_result_to_exh exh Match_type_error r ⇔ r = Match_type_error)`,
+ rw [] >>
+ cases_on `r` >>
+ rw [match_result_to_exh_def]);
+
+val match_result_nomatch = Q.prove (
+`(!exh r. match_result_to_exh exh r No_match ⇔ r = No_match) ∧
+ (!exh r. match_result_to_exh exh No_match r ⇔ r = No_match)`,
+ rw [] >>
+ cases_on `r` >>
+ rw [match_result_to_exh_def]);
+
+val pmatch_exh_correct = Q.prove (
+`(!exh s p v env r env_exh s_exh v_exh.
+  r ≠ Match_type_error ∧
+  pmatch_i2 exh s p v env = r ∧
+  vs_to_exh exh s s_exh ∧
+  v_to_exh exh v v_exh ∧
+  env_to_exh exh env env_exh
+  ⇒
+  ?r_exh.
+    pmatch_exh s_exh (pat_to_exh p) v_exh env_exh = r_exh ∧
+    match_result_to_exh exh r r_exh) ∧
+ (!exh s ps vs env r env_exh s_exh vs_exh.
+  r ≠ Match_type_error ∧
+  pmatch_list_i2 exh s ps vs env = r ∧
+  vs_to_exh exh s s_exh ∧
+  vs_to_exh exh vs vs_exh ∧
+  env_to_exh exh env env_exh
+  ⇒
+  ?r_exh.
+    pmatch_list_exh s_exh (MAP pat_to_exh ps) vs_exh env_exh = r_exh ∧
+    match_result_to_exh exh r r_exh)`,
+ ho_match_mp_tac pmatch_i2_ind >>
+ rw [pmatch_i2_def, pmatch_exh_def, pat_to_exh_def, match_result_to_exh_def] >>
+ fs [match_result_to_exh_def, bind_def, v_to_exh_eqn] >>
+ rw [pmatch_exh_def, match_result_to_exh_def, match_result_error] >>
+ imp_res_tac LIST_REL_LENGTH >>
+ fs []
+ >- metis_tac []
+ >- (every_case_tac >>
+     fs [] >>
+     metis_tac [])
+ >- (every_case_tac >>
+     fs [] >>
+     metis_tac [])
+ >- (every_case_tac >>
+     fs [match_result_to_exh_def])
+ >- metis_tac []
+ >- (every_case_tac >>
+     fs [match_result_error, store_lookup_def, LIST_REL_EL_EQN] >>
+     metis_tac [])
+ >- (every_case_tac >>
+     rw [match_result_to_exh_def] >>
+     res_tac >>
+     fs [match_result_nomatch] >>
+     cases_on `pmatch_exh s_exh (pat_to_exh p) y env_exh` >>
+     fs [match_result_to_exh_def] >>
+     metis_tac []));
 
 val pat_bindings_exh_correct = prove(
   ``(∀p ls. pat_bindings_exh (pat_to_exh p) ls = pat_bindings_i2 p ls) ∧
@@ -285,9 +399,9 @@ val exp_to_exh_correct = Q.store_thm ("exp_to_exh_correct",
                           (pat_exp_to_exh exh pes')
                           (result_to_exh v_to_exh exh r))`,
  ho_match_mp_tac evaluate_i3_ind >>
- rw [exp_to_exh_def, v_to_exh_def, result_to_exh_def] >>
+ rw [exp_to_exh_def, v_to_exh_eqn, result_to_exh_def] >>
  ONCE_REWRITE_TAC [evaluate_exh_cases] >>
- fs [v_to_exh_def, result_to_exh_def, store_to_exh_def] >>
+ fs [v_to_exh_eqn, result_to_exh_def, store_to_exh_def] >>
  TRY (Cases_on `err`) >>
  fs [] >>
  rw []
@@ -297,51 +411,51 @@ val exp_to_exh_correct = Q.store_thm ("exp_to_exh_correct",
  >- (induct_on `env` >>
      rw [] >>
      PairCases_on `h` >>
-     fs [v_to_exh_def] >>
+     fs [v_to_exh_eqn] >>
      rw [] >>
      fs [])
  >- (`n < LENGTH genv` by decide_tac >>
      rw [EL_MAP])
  >- (fs [do_uapp_exh_def, do_uapp_i3_def] >>
      every_case_tac >>
-     fs [v_to_exh_def] >>
+     fs [v_to_exh_eqn] >>
      rw []
      >- (MAP_EVERY qexists_tac [`Loc_exh n`, `MAP (v_to_exh exh) s2`] >>
          rw [] >>
          fs [store_lookup_def, EL_MAP])
      >- (fs [LET_THM, store_alloc_def] >>
-         rw [v_to_exh_def])
+         rw [v_to_exh_eqn])
      >- (MAP_EVERY qexists_tac [`v_to_exh exh v`, `MAP (v_to_exh exh) s2`, `MAP (OPTION_MAP (v_to_exh exh)) genv2`] >>
-         rw [LUPDATE_MAP, EL_MAP, v_to_exh_def]))
+         rw [LUPDATE_MAP, EL_MAP, v_to_exh_eqn]))
  >- (disj1_tac >>
      first_assum(match_exists_tac o concl) >> simp[] >>
      first_assum(match_exists_tac o concl) >> simp[] >>
      fs[do_app_i2_def] >>
      every_case_tac >>
-     fs[do_app_exh_def,v_to_exh_def,do_eq_i2_def] >>
+     fs[do_app_exh_def,v_to_exh_eqn,do_eq_i2_def] >>
      rw[] >> fs[] >>
      fs[exp_to_exh_def,exn_env_i2_def] >>
-     fs[v_to_exh_def,bind_def,emp_def] >>
+     fs[v_to_exh_eqn,bind_def,emp_def] >>
      fs[store_assign_def,evaluate_exh_lit] >>
-     rw[LUPDATE_MAP,v_to_exh_def] >>
+     rw[LUPDATE_MAP,v_to_exh_eqn] >>
      fs[funs_to_exh_MAP,MAP_MAP_o,combinTheory.o_DEF,UNCURRY,FST_triple,ETA_AX])
  >- (disj1_tac >>
      first_assum(match_exists_tac o concl) >> simp[] >>
      first_assum(match_exists_tac o concl) >> simp[] >>
      fs[do_app_i2_def] >>
      every_case_tac >>
-     fs[do_app_exh_def,v_to_exh_def,do_eq_i2_def] >>
+     fs[do_app_exh_def,v_to_exh_eqn,do_eq_i2_def] >>
      rw[] >> fs[] >>
      fs[exp_to_exh_def,exn_env_i2_def] >>
-     fs[v_to_exh_def,bind_def,emp_def] >>
+     fs[v_to_exh_eqn,bind_def,emp_def] >>
      fs[store_assign_def,evaluate_exh_lit] >>
-     rw[LUPDATE_MAP,v_to_exh_def] >>
+     rw[LUPDATE_MAP,v_to_exh_eqn] >>
      fs[funs_to_exh_MAP,MAP_MAP_o,combinTheory.o_DEF,UNCURRY,FST_triple,ETA_AX])
  >- (disj2_tac >> disj1_tac >>
      first_assum(match_exists_tac o concl) >> simp[] >>
      first_assum(match_exists_tac o concl) >> simp[] >>
      fs[do_app_i2_def] >>
-     every_case_tac >> fs[v_to_exh_def,do_app_exh_def] >>
+     every_case_tac >> fs[v_to_exh_eqn,do_app_exh_def] >>
      fs[funs_to_exh_MAP,MAP_MAP_o,combinTheory.o_DEF,UNCURRY,FST_triple,ETA_AX])
  >- metis_tac []
  >- metis_tac []
@@ -353,7 +467,7 @@ val exp_to_exh_correct = Q.store_thm ("exp_to_exh_correct",
      fs [] >>
      disj1_tac >>
      first_assum(match_exists_tac o concl) >> simp[] >>
-     simp[v_to_exh_def])
+     simp[v_to_exh_eqn])
  >- (res_tac >>
      fs [] >>
      cases_on `exhaustive_match exh (MAP FST pes)` >>
@@ -362,7 +476,7 @@ val exp_to_exh_correct = Q.store_thm ("exp_to_exh_correct",
  >- (
    disj1_tac >>
    first_assum(match_exists_tac o concl) >> simp[] >>
-   fs[opt_bind_def] >> every_case_tac >> fs[v_to_exh_def] )
+   fs[opt_bind_def] >> every_case_tac >> fs[v_to_exh_eqn] )
  >- (
    simp[funs_to_exh_MAP,MAP_MAP_o,combinTheory.o_DEF,UNCURRY] >>
    fs[ETA_AX,FST_triple] )
@@ -377,7 +491,7 @@ val exp_to_exh_correct = Q.store_thm ("exp_to_exh_correct",
      ONCE_REWRITE_TAC [evaluate_exh_cases] >>
      rw [] >>
      ONCE_REWRITE_TAC [evaluate_exh_cases] >>
-     rw [v_to_exh_def] >>
+     rw [v_to_exh_eqn] >>
      ONCE_REWRITE_TAC [evaluate_exh_cases] >>
      rw [lookup_def,bind_def] >>
      CONV_TAC SWAP_EXISTS_CONV >>
